\subsection{Flow equation}\label{sec:equation}

Consider an infinitesimal generating process on a Riemannian surface $M$ using two generators:
one for an additional action $\mu$ and the other for a multiplicative action $e^\lambda$.
These two generators are perpendicular.
This generation process produces an assignment $A: M \to R$ over the surface.

For any point with an assignment $a_0$, if we consider a movement of distance $\epsilon$ in a direction with angle $\theta$
over a time period of $\delta$, we can establish the following:

\[
    a_{\delta} = (a_0 + \mu \epsilon \cos \theta)e^{\lambda \epsilon \sin \theta}
\]

or

\[
    a_{\delta} = a_0 e^{\lambda \epsilon \sin \theta} + \mu \epsilon \cos \theta
\]

Both formula can be simplified to the same result:

\[
    a_{\delta} = a_0 + \epsilon (a_0 \lambda \sin \theta + \mu \cos \theta)
\]

Then, we have the following equation:

\[
    \frac{1}{\delta} (a_{\delta} - a_0) = \frac{\epsilon}{\delta} (\mu \cos \theta + x_0 \lambda \sin \theta)
\]

When both $\delta$ and $\epsilon$ are towards zero, we get $da / dt$, and hence

\[
    \frac{da}{dt} = u (\mu \cos \theta + a \lambda \sin \theta)
\]

Or, we can change it to another form

\begin{equation}
    \frac{da}{ds} = \mu \cos \theta + a \lambda \sin \theta\label{eq:flow}
\end{equation}

We name this equation~\eqref{eq:flow} as the flow equation.

The left side of this equation is governed by the distance structure, while the right side is governed by the angle structure.
This leads to below theorem.

\begin{theorem}
Isometries keep the flow equation\eqref{eq:flow}
\label{thm:isometry}
\end{theorem}

\begin{proof}
  An isometry keeps both the distance structure and the angle structure, so it keeps the flow equation.
\end{proof}

We can also get a direct formal solution of the flow equation~\eqref{eq:flow}(details in Appendix~\ref{sec:directformalsolution}).

\begin{equation}
   a = (a_0 + \frac{\mu}{\lambda} \cot \theta) e^{\lambda s \sin \theta} - \frac{\mu}{\lambda} \cot \theta\label{eq:solution}
\end{equation}

While the validity of this solution is still uncertain because we have not assumed any constraints on the local coordinate system,
it is still a useful starting point for further investigation.
For example, we can use this solution to derive (details in Appendix~\ref{sec:conformance}) the relationship between assignments at different vertices in a cell of a mesh grid.

Assuming the assignment at the center point of a cell is $a_0$, we move in different directions and obtain the following assignments:

\begin{itemize}
\item $\theta = 0$: $a_s = a_0 + \mu s$
\item $\theta = \frac{\pi}{2}$: $a_s = a_0 e^{\lambda s}$
\item $\theta = \pi$: $a_s = a_0 - \mu s$
\item $\theta = \frac{3 \pi}{2}$: $a_s = a_0 e^{- \lambda s} $
\end{itemize}

This result is straightforward, but it demonstrates that the infinitesimal generating process is consistent with the discrete mesh grid.

\subsection{The contour-gradient form of flow equation}\label{subsec:the-contour-gradient-form}

It is easy to derive the contour equation in the local coordinate

\begin{equation}
    \mu \cos \theta_c + a \lambda \sin \theta_c = 0\label{eq:contour}
\end{equation}

then we have

\begin{equation}
    \theta_c = - \arctan \frac{\mu}{a \lambda}\label{eq:contourangle}
\end{equation}

the contour and the gradient are perpendicular to each other

\begin{equation}
    \theta_g = \pm \frac{\pi}{2} - \arctan \frac{\mu}{a \lambda}\label{eq:gradientangle}
\end{equation}

then along $\theta_g$ we have

\begin{equation}
    \frac{da}{ds} = \mu \cos (\pm \frac{\pi}{2} - \arctan \frac{\mu}{a \lambda}) + a \lambda \sin (\pm \frac{\pi}{2} - \arctan \frac{\mu}{a \lambda})
    \label{eq:alonggradient}
\end{equation}

\begin{equation}
    \frac{da}{ds} = \pm \sqrt{\mu^2 + \lambda^2 a^2}\label{eq:grad}
\end{equation}

By introducing the right-hand rotation angle $\phi$ along the gradient direction, we can establish a local polar coordinate system based on the gradient and contour lines.
Then the growth rate of $a$ along the angle $\phi$ is

\begin{equation}
    \frac{da}{ds} = \mu \cos (\frac{\pi}{2} - \arctan \frac{\mu}{a \lambda} + \phi) + a \lambda \sin (\frac{\pi}{2} - \arctan \frac{\mu}{a \lambda} + \phi)
    \label{eq:fourfold}
\end{equation}

And the simplified equation is

\begin{equation}
    \frac{da}{ds} = \sqrt {\mu^2 + a^2 \lambda^2} \cos \phi\label{eq:contourgradient}
\end{equation}

or

\begin{equation}
    \frac{da_{\phi}}{ds_{\phi}} = \sqrt {\mu^2 + a^2 \lambda^2} \cos \phi\label{eq:contourgradient2}
\end{equation}

if we want to emphasize the path is along the angle $\phi$.

The equation~\eqref{eq:contourgradient} is the flow equation in the contour-gradient coordinate system.

Equation~\eqref{eq:contourgradient} is solvable, and we get the relation between $a$ and $s$:

\begin{equation}\label{eq:rel_a_s}
    \tanh(\lambda s \cos \phi - c) = \frac{\lambda a}{\sqrt{\mu^2 + \lambda^2 a^2}}
\end{equation}

we can further simplify the equation to

\begin{equation}
  a = \pm \frac{\mu}{\lambda} \sinh(\lambda s \cos \phi - c)\label{eq:gradevo}
\end{equation}

Under the initial condition $a = a_0$ when $s = 0$, we can get the following equation:

\begin{equation}
    a = \frac{\mu}{\lambda} \sinh(\lambda s \cos \phi + \arcsinh \frac{a_0 \lambda}{\mu})\label{eq:gradevo2}
\end{equation}

or

\begin{equation}
    a = - \frac{\mu}{\lambda} \sinh(\lambda s \cos \phi - \arcsinh \frac{a_0 \lambda}{\mu})\label{eq:gradevo3}
\end{equation}

In this coordinate system, the additional line and the multiplicative line are:

\begin{equation}
    \phi = \arccos \frac{\mu}{\sqrt {\mu^2 + a^2 \lambda^2}} \label{eq:additionalline}
\end{equation}

\begin{equation}
    \phi = \arcsin \frac{\mu}{\sqrt {\mu^2 + a^2 \lambda^2}}\label {eq:mulitiplcativeline}
\end{equation}

\subsection{Flow and function}\label{subsec:flow-and-function}

In this section, we aim to present novel insight into functions.
Namely, the treatment of functions as flows will be discussed.

\begin{definition}\label{def:projection}
Given a function $k$ on the real domain $R$, we can introduce a mapping $l$ on the arithmetic expression space $H$ such that the following diagram commutes.

\begin{center}
    \begin{tikzcd}
        H && H \\
        R && R
        \arrow["l", from=1-1, to=1-3]
        \arrow["\nu"', from=1-1, to=2-1]
        \arrow["\nu", from=1-3, to=2-3]
        \arrow["k"', from=2-1, to=2-3]
    \end{tikzcd}
\end{center}

where $\nu$ is the evaluation function of the expression. Then we call the mapping $l$ is the promotion of the function $k$,
or function $k$ is the projection of the mapping $l$.
\end{definition}

A mapping $l$ on the arithmetic expression space $H$ can be implemented by a geometry flow on $M$.
We give an example of function $\sin$ as follows.

\subsubsection{The flow of sine}\label{subsubsec:flow-of-sine}

Form the flow equation~\eqref{eq:flow} we have

$$\frac{da}{ds} = \cos \theta + a \sin \theta$$

$$\frac{da}{dt} = (\cos \theta + a \sin \theta)\frac{ds}{dt}$$

And along the variation of $t$, we have $a(t) = \sin t$, so we have

$$\cos t = (\cos \theta + \sin t \sin \theta)\frac{ds}{dt}$$

$$\frac{ds}{dt} = \frac{\cos t}{\cos \theta + \sin t \sin \theta}$$

\subsubsection{Brachistochrone curve}\label{subsubsec:brachistochrone}

The brachistochrone curve is the curve between two points that minimizes the time taken by a frictionless bead sliding along a wire.
We assume the wire is a curve $\eta = f(\delta)$, and the bead starts at $(0, 0)$ and ends at $( \Delta, H )$ as time $t$ goes from $0$ to $T$.

\subsection{The existence theorems}\label{subsec:existence-theorems}

There are two important existence theorems related to the flow equation~\eqref{eq:flow}.

The first existence theorem states that if we have a Riemann surface $M$, then there exists a function $a$ on $M$ that satisfies the flow equation~\eqref{eq:flow}. This theorem is proved in a later section, and we will not go into the details of the proof here.

\begin{theorem}
    Given a 2D Riemannian manifold $M$, there exists a function $a$ on $M$ satisfying the flow equation~\eqref{eq:flow}.
    \label{prop:existence1st}
\end{theorem}

The second existence theorem is also crucial.
It says that if we have a smooth surface $S$ and a function $a$ on $S$, then we can find a metric $g$ on $S$ that makes $a$ satisfy the flow equation~\eqref{eq:flow}.

\begin{theorem}(By Le Zhang)
    Given an oriented 2D Riemannian manifold $S$, and a function $a$ over $S$, there exists a metric $g$ on $S$ that makes $a$
    satisfying the flow equation~\eqref{eq:flow}.
    \label{prop:existence2nd}
\end{theorem}

\begin{proof}
    The proof consists of two main steps. First, we demonstrate the existence of a metric \( g \) on \( S \) that allows \( a \) to satisfy the flow equation~\eqref{eq:flow} in a local coordinate system. Then, we show that this local metric can be extended to a global metric on \( S \).

    \emph{Part 1: Local Perspective}

    Consider a point \( p \) on the surface \( S \), and there is a neighborhood \( U \) around \( p \).
    In this area, we can find a local isothermal coordinate system in which the metric takes the form:
    \[ ds^2 = e^{2\rho}(du^2 + dv^2), \]
    where \( u \) and \( v \) are the coordinates of \( U \), and \( \rho \) is a function of \( u, v \) in \( U \).
    The gradient of \( a \) in this local isothermal coordinate system is expressed as:
    \[ \nabla a = \frac{\partial a}{\partial u} du + \frac{\partial a}{\partial v} dv. \]
    Using the definition of the directional derivative, we obtain:
    \[ \frac{da_{\psi}}{ds_{\psi}} = ||\nabla a|| \cos \psi, \]
    where \( ||\nabla a|| \) is the norm of \( \nabla a \), and \( \psi \) is the angle between \( \nabla a \) and the direction of movement.

    Now, considering the flow equation~\ref{eq:contourgradient2} in the gradient-contour coordinate system, we have:
    \[ \frac{da_{\phi}}{ds_{\phi}} = \sqrt{\mu^2 + a^2 \lambda^2} \cos \phi. \]

    Note that \( ||\nabla a|| \) is fixed for the given function \( a \) and the local coordinate system, and \( \sqrt{\mu^2 + a^2 \lambda^2} \) is also fixed for the given function \( a \).
    We can scale \( e^{2\rho} \) with a linear factor \( \kappa \) to make \( ||\nabla a|| \) match the fixed value of \( \sqrt{\mu^2 + a^2 \lambda^2} \),
    thus we have a morphing process controlled by \( \kappa \) that
    \begin{align}
    ds^2 &= \kappa e^{2 \rho}(du^2 + dv^2)\label{eq:morphing} \\
         &= e^{2 \rho + \ln \kappa}(du^2 + dv^2).
    \end{align}

    Under the morphing ratio \( \kappa \), we have:

    \begin{equation}
      ||\nabla_\kappa a|| = \kappa^{-1} ||\nabla a||,
    \end{equation}

    and when \( \kappa \) is set to the value of:

    \[ ||\nabla_\kappa a|| = \sqrt{\mu^2 + a^2 \lambda^2}, \]

    the flow equation~\eqref{eq:flow} is satisfied in the local coordinate system.

    The morphing ratio \( \kappa \) is calculated as follows:
    \begin{equation}
        \kappa = \frac{||\nabla a||}{\sqrt{\mu^2 + a^2 \lambda^2}}\label{eq:ratio}.
    \end{equation}

    \emph{Part 2: Global Perspective}

    \qedhere
\end{proof}

\subsection{Notion study}\label{subsec:notion-study}

The flow equation~\eqref{eq:flow} is taken in a local polar coordinate system,

$$\frac{da}{ds} = \mu \cos \theta + a \lambda \sin \theta$$

If we take $dx = \cos \theta ds$ and $dy = \sin \theta ds$, we can rewrite it as

$$da = \mu dx + a \lambda dy$$

$$a + da = (a + \mu dx)e^{\lambda dy}$$

$$a + da = (a + \mu dx)e^{\lambda dy}$$

$$\lfloor a \rfloor = \lceil \lfloor A \rfloor \rceil $$
