
In order to verify the conformance, we expand the formula \eqref{eq:directformalsolution} in the following way:

\begin{equation}
   a =  a_0 e^{\lambda s \sin \theta} + \frac{\mu}{\lambda} [1 + \lambda s \sin \theta + \frac{1}{2!} (\lambda s \sin \theta)^2  + \frac{1}{3!} (\lambda s \sin \theta)^3 + \cdots - 1] \cot \theta
\end{equation}

\begin{equation}
   a = a_0 e^{\lambda s \sin \theta} + \mu s \cos \theta + \frac{\mu}{\lambda} \sin \theta \cos \theta (\frac{\lambda^2s^2}{2!} + \frac{\lambda^3s^3}{3!} \sin \theta + \frac{\lambda^4s^4}{4!} \sin^2 \theta + \cdots)
\end{equation}

\begin{equation}
   a = a_0 e^{\lambda s \sin \theta} + \mu s \cos \theta + \frac{\mu}{2\lambda} \sin 2\theta (\frac{\lambda^2s^2}{2!} + \frac{\lambda^3s^3}{3!} \sin \theta + \frac{\lambda^4s^4}{4!} \sin^2 \theta + \cdots)
\end{equation}

\begin{equation}
   a = a_0 e^{\lambda s \sin \theta} + \mu s \cos \theta + \frac{\mu}{2\lambda} \Psi(s) \sin 2\theta
\end{equation}

When $\theta = \frac{k \pi}{2}, k = 0, 1, 2, 3\cdots, s = 0, 1, 2, 3\cdots$, we have

\begin{equation}
    a = a_0 e^{\lambda s \sin \theta} + \mu s \cos \theta
\end{equation}

Especially, we have

\begin{equation}
    a = a_0 + \mu s, s = 0, 1, 2, 3\cdots, k = 0, 1, 2, 3\cdots, \theta = 2k\pi
\end{equation}

\begin{equation}
    a = x_0e^{\lambda s}, s = 0, 1, 2, 3\cdots, k = 0, 1, 2, 3\cdots, \theta = 2k\pi + \frac{\pi}{2}
\end{equation}

\begin{equation}
    a = a_0 - \mu s, s = 0, 1, 2, 3\cdots, k = 0, 1, 2, 3\cdots, \theta = 2k\pi + \pi
\end{equation}

\begin{equation}
    a = a_0 e^{- \lambda s}, s = 0, 1, 2, 3\cdots, k = 0, 1, 2, 3\cdots, \theta = 2k\pi + \frac{3 \pi}{2}
\end{equation}

which gives the conformance.

