
We can also get a direct formal solution of the flow equation (\eqref{eq:flow}) step by step:

$$
    \frac{da}{\mu \cos \theta + a \lambda \sin \theta} = ds
$$

$$
    \frac{1}{\lambda \sin \theta} \frac{d(\mu \cos \theta + a \lambda \sin \theta)}{\mu \cos \theta + a \lambda \sin \theta} = ds
$$

$$
    \frac{1}{\lambda \sin \theta} ln(\mu \cos \theta + a \lambda \sin \theta) = s + C
$$

$$
    \mu \cos \theta + a \lambda \sin \theta = e^{\lambda s \sin \theta} e^{C \lambda \sin \theta}
$$

Considering the initial condition
$$
    \mu \cos \theta + a_0 \lambda \sin \theta = e^{C \lambda \sin \theta}
$$

We have
$$
    \mu \cos \theta + a \lambda \sin \theta = e^{\lambda s \sin \theta} (\mu \cos \theta + a_0 \lambda \sin \theta)
$$

$$
   a = \frac{\mu \cos \theta + a_0 \lambda \sin \theta}{\lambda \sin \theta} e^{\lambda s \sin \theta} - \frac{\mu}{\lambda}\cot \theta
$$

$$
   a = (a_0 + \frac{\mu}{\lambda} \cot \theta) e^{\lambda s \sin \theta} - \frac{\mu}{\lambda} \cot \theta
$$

\begin{equation}
   a =  a_0 e^{\lambda s \sin \theta} + \frac{\mu}{\lambda} (e^{\lambda s \sin \theta} - 1) \cot \theta
\end{equation}

\begin{equation}\label{eq:directformalsolution}
   a =  a_0 e^{\lambda s \sin \theta} + \frac{\mu}{\lambda} (e^{\lambda s \sin \theta} - 1) \cot \theta
\end{equation}

